# This is a draft RDF vocabulary for representing spatial data sets in INSPIRE as RDF. This vocabulary has been created using the "Guidelines for the RDF encoding of spatial data" (http://inspire-eu-rdf.github.io/inspire-rdf-guidelines).
#
# The use of RDF is optional and does not supersede or replace the requirements regarding encoding specified in Clause 9 of the INSPIRE Data Specifications. This optional encoding is intended to support the e-government and open data community in Europe, which is increasingly looking at RDF to represent data.
#
# This is a draft version. It has limitations and is expected to contain errors. Please report any issues or concerns in GitHub (https://github.com/inspire-eu-rdf/inspire-rdf-vocabularies/issues).
#
# ------------------------------
#
#
# This ontology contains classes and properties that have been derived from the INSPIRE "CadastralParcels" application schema.
#
# The following properties have been encoded with global scope (see guidelines for further details):
#  - CadastralParcel.referencePoint
#
# During the derivation, the following mappings, alignments, and omissions have been applied:
# - Mappings:
#   - Code lists are mapped to skos:Concept.
#   - The properties 'beginLifespanVersion', 'endLifespanVersion', 'validFrom', and 'validTo' are mapped to the global properties defined by the base ontology.
#   - Geometry types are mapped to classes from the Simple Feature ontology.
#   - Property 'label' is mapped to rdfs:label.
#   - Property 'CadastralZoning.referencePoint' is mapped to the global property 'referencePoint' from this ontology.
#
# - Alignments (through subsumption):
#   - Spatial object types are aligned with gsp:Feature.
#   - Properties with value type 'GeographicalName' are aligned to property locn:geographicName.
#   - Properties 'CadastralParcel.geometry', 'CadastralBoundary.geometry', and 'CadastralZoning.geometry' are aligned to locn:geometry and gsp:hasDefaultGeometry.
#   - Property 'CadastralParcel.referencePoint'is aligned to locn:geometry and gsp:hasGeometry.
#
# - Omissions:
#   - Property 'inspireId' is omitted. See the guidelines for further details.
#
# ------------------------------
#
#
@prefix au:    <http://inspire.ec.europa.eu/ont/au#> .
@prefix iso19150-2: <http://def.isotc211.org/iso19150-2/2012/base#> .
@prefix rdf:   <http://www.w3.org/1999/02/22-rdf-syntax-ns#> .
@prefix gsp:   <http://www.opengis.net/ont/geosparql#> .
@prefix owl:   <http://www.w3.org/2002/07/owl#> .
@prefix gn:    <http://inspire.ec.europa.eu/ont/ad#> .
@prefix xsd:   <http://www.w3.org/2001/XMLSchema#> .
@prefix skos:  <http://www.w3.org/2004/02/skos/core#> .
@prefix rdfs:  <http://www.w3.org/2000/01/rdf-schema#> .
@prefix locn:  <https://www.w3.org/ns/locn#> .
@prefix cp:    <http://inspire.ec.europa.eu/ont/cp#> .
@prefix base:  <http://inspire.ec.europa.eu/ont/base#> .

cp:CadastralParcel.administrativeUnit
        a                owl:ObjectProperty ;
        rdfs:domain      cp:CadastralParcel ;
        rdfs:range       au:AdministrativeUnit ;
        skos:definition  "The administrative unit of lowest administrative level containing this cadastral parcel."@en .

cp:CadastralZoning.estimatedAccuracy
        a                owl:DatatypeProperty ;
        rdfs:comment     "NOTE This mean value may come from quality measures on a homogeneous population of cadastral parcels or from an estimation based on the knowledge of the production processes and of their accuracy."@en ;
        rdfs:domain      cp:CadastralZoning ;
        rdfs:range       base:Measure ;
        skos:definition  "The estimated absolute positional accuracy of cadastral parcels within the cadastral zoning in the used INSPIRE coordinate reference system. Absolute positional accuracy is the mean value of the positional uncertainties for a set of positions, where the positional uncertainties are the distance between a measured position and what is considered as the corresponding true position."@en .

cp:BasicPropertyUnit.areaValue
        a                owl:DatatypeProperty ;
        rdfs:domain      cp:BasicPropertyUnit ;
        rdfs:range       base:Measure ;
        skos:definition  "Registered area value giving quantification of the area projected on the horizontal plane of the cadastral parcels composing the basic property unit."@en .

cp:CadastralZoning.levelName
        a                owl:DatatypeProperty ;
        rdfs:comment     "EXAMPLE  For Spain, level name might be supplied as \"municipio\" (in Spanish) and as \"municipality\" (in English)."@en ;
        rdfs:domain      cp:CadastralZoning ;
        rdfs:range       rdf:langString ;
        skos:definition  "Name of the level of the cadastral zoning in the national cadastral hierarchy, in at least one official language of the European Union."@en .

cp:BasicPropertyUnit  a        owl:Class ;
        rdfs:comment           "SOURCE Adapted from UN ECE 2004.\r\n\r\nNOTE 1 In the INSPIRE context, basic property units are to be made available by member states where unique cadastral references are given only for basic property units and not for parcels.\r\n\r\nNOTE 2 In many (but not all) countries, the area of the basic property unit corresponds to the cadastral parcel itself.\r\n\r\nNOTE 3 Some countries, such as Finland, may also register officially basic property units without any area. These basic property units are considered out of the INSPIRE scope.\r\n\r\nNOTE 4 Some countries, such as Norway, may have parcels which belong to several basic property units."@en ;
        rdfs:isDefinedBy       <http://inspire.ec.europa.eu/featureconcept/BasicPropertyUnit> ;
        rdfs:subClassOf        gsp:Feature ;
        iso19150-2:constraint  "validTo: /* If set, the date validTo shall be equal or later than validFrom. */" , "endLifespanVersion: /* If set, the date endLifespanVersion shall be later than beginLifespanVersion. */" , "areaValueUoM: /* Value of areaValue shall be given in square meters */" ;
        skos:definition        "The basic unit of ownership that is recorded in the land books, land registers or equivalent. It is defined by unique ownership and homogeneous real property rights, and may consist of one or more adjacent or geographically separate parcels."@en .

cp:CadastralParcel.basicPropertyUnit
        a                owl:ObjectProperty ;
        rdfs:domain      cp:CadastralParcel ;
        rdfs:range       cp:BasicPropertyUnit ;
        skos:definition  "The basic property unit(s) containing this cadastral parcel."@en .

cp:CadastralBoundary.geometry
        a                   owl:ObjectProperty ;
        rdfs:domain         cp:CadastralBoundary ;
        rdfs:range          gsp:Geometry ;
        rdfs:subPropertyOf  locn:geometry , gsp:hasDefaultGeometry ;
        skos:definition     "Geometry of the cadastral boundary."@en .

cp:CadastralParcel.geometry
        a                   owl:ObjectProperty ;
        rdfs:comment        "As much as possible, the geometry should be a single area."@en ;
        rdfs:domain         cp:CadastralParcel ;
        rdfs:range          gsp:Geometry ;
        rdfs:subPropertyOf  locn:geometry , gsp:hasDefaultGeometry ;
        skos:definition     "Geometry of the cadastral parcel."@en .

cp:BasicPropertyUnit.administrativeUnit
        a                owl:ObjectProperty ;
        rdfs:domain      cp:BasicPropertyUnit ;
        rdfs:range       au:AdministrativeUnit ;
        skos:definition  "The administrative unit of lowest administrative level containing this basic property unit."@en .

cp:CadastralParcel.nationalCadastralReference
        a                owl:DatatypeProperty ;
        rdfs:comment     "The national cadastral reference can be used also in further queries in national services."@en ;
        rdfs:domain      cp:CadastralParcel ;
        rdfs:range       xsd:string ;
        skos:definition  "Thematic identifier at national level, generally the full national code of the cadastral parcel. Must ensure the link to the national cadastral register or equivalent."@en .

cp:CadastralZoning.level
        a                owl:ObjectProperty ;
        rdfs:domain      cp:CadastralZoning ;
        rdfs:range       skos:Concept ;
        rdfs:seeAlso     <http://inspire.ec.europa.eu/codelist/CadastralZoningLevelValue> ;
        skos:definition  "Level of the cadastral zoning in the national cadastral hierarchy."@en .

cp:referencePoint  a        owl:ObjectProperty , rdf:Property ;
        rdfs:comment        "EXAMPLE The centroid of the cadastral parcel geometry."@en ;
        rdfs:range          gsp:Geometry ;
        rdfs:subPropertyOf  locn:geometry , gsp:hasGeometry ;
        skos:definition     "A point within the cadastral parcel."@en .

cp:CadastralParcel.zoning
        a                owl:ObjectProperty ;
        rdfs:domain      cp:CadastralParcel ;
        rdfs:range       cp:CadastralZoning ;
        skos:definition  "The cadastral zoning of lowest level containing this cadastral parcel."@en .

cp:CadastralZoning.originalMapScaleDenominator
        a                owl:DatatypeProperty ;
        rdfs:comment     "EXAMPLE 2000 means that original cadastral map was designed at scale 1: 2000."@en ;
        rdfs:domain      cp:CadastralZoning ;
        rdfs:range       xsd:integer ;
        skos:definition  "The denominator in the scale of the original paper map (if any) to whose extent the cadastral zoning corresponds."@en .

cp:CadastralBoundary  a        owl:Class ;
        rdfs:comment           "NOTE In the INSPIRE context, cadastral boundaries are to be made available by member states where absolute positional accuracy information is recorded for the cadastral boundary (attribute estimated accuracy)."@en ;
        rdfs:isDefinedBy       <http://inspire.ec.europa.eu/featureconcept/CadastralBoundary> ;
        rdfs:subClassOf        gsp:Feature ;
        iso19150-2:constraint  "validTo: /* If set, the date validTo shall be equal or later than validFrom. */" , "estimatedAccuracyUoM: /* Value of estimatedAccuracy shall be given in meters. */" , "endLifespanVersion: /* If set, the date endLifespanVersion shall be later than beginLifespanVersion. */\r\n" ;
        skos:definition        "Part of the outline of a cadastral parcel. One cadastral boundary may be shared by two neighbouring cadastral parcels."@en .

cp:BasicPropertyUnit.nationalCadastralReference
        a                owl:DatatypeProperty ;
        rdfs:comment     "The national cadastral reference can be used also in further queries in national services."@en ;
        rdfs:domain      cp:BasicPropertyUnit ;
        rdfs:range       xsd:string ;
        skos:definition  "Thematic identifier at national level, generally the full national code of the basic property unit. Must ensure the link to the national cadastral register or equivalent."@en .

cp:CadastralZoning.upperLevelUnit
        a                owl:ObjectProperty ;
        rdfs:domain      cp:CadastralZoning ;
        rdfs:range       cp:CadastralZoning ;
        skos:definition  "The next upper level cadastral zoning containing this cadastral zoning."@en .

cp:CadastralParcel  a          owl:Class ;
        rdfs:comment           "SOURCE [INSPIRE Directive:2007].\r\n\r\nNOTE As much as possible, in the INSPIRE context, cadastral parcels should be forming a partition of national territory. Cadastral parcel should be considered as a single area of Earth surface (land and/or water), under homogeneous real property rights and unique ownership, real property rights and ownership being defined by national law (adapted from UN ECE 2004 and WG-CPI, 2006). By unique ownership is meant that the ownership is held by one or several joint owners for the whole parcel."@en ;
        rdfs:isDefinedBy       <http://inspire.ec.europa.eu/featureconcept/CadastralParcel> ;
        rdfs:subClassOf        gsp:Feature ;
        iso19150-2:constraint  "validTo: /* If set, the date validTo shall be equal or later than validFrom. */" , "geometryType: Type of geometry shall be GM_Surface or GM_MultiSurface" , "endLifespanVersion: /* If set, the date endLifespanVersion shall be later than beginLifespanVersion. */" , "areaValueUoM: /* Value of areaValue shall be given in square meters. */" ;
        skos:definition        "Areas defined by cadastral registers or equivalent."@en .

cp:CadastralParcel.areaValue
        a                owl:DatatypeProperty ;
        rdfs:domain      cp:CadastralParcel ;
        rdfs:range       base:Measure ;
        skos:definition  "Registered area value giving quantification of the area projected on the horizontal plane of the cadastral parcel."@en .

<http://inspire.ec.europa.eu/ont/cp>
        a                owl:Ontology ;
        owl:imports      <http://def.isotc211.org/iso19150-2/2012/base> , <https://github.com/inspire-eu-rdf/inspire-rdf-vocabularies/blob/master/ad/ad.ttl> , <https://www.w3.org/ns/locn.ttl> , <http://www.w3.org/2004/02/skos/core> , <http://www.opengis.net/ont/geosparql> , <https://github.com/inspire-eu-rdf/inspire-rdf-vocabularies/blob/master/base/base.ttl> , <https://github.com/inspire-eu-rdf/inspire-rdf-vocabularies/blob/master/au/au.ttl> ;
        owl:versionIRI   "http://inspire.ec.europa.eu/ont/cp/4.0" ;
        owl:versionInfo  "4.0" ;
        skos:definition  "The application schema CadastralParcels contains the feature types CadastralParcel, CadastralBoundary and CadastralIndexSet."@en .

cp:CadastralZoning.name
        a                   owl:ObjectProperty ;
        rdfs:comment        "NOTE 1 Cadastral zonings which are also administrative units have generally a name.\r\n\r\nEXAMPLE Bordeaux, Copenhagen.\r\n\r\nNOTE 2 The language of the name should be filled in most cases, except if the data producer does not know in which language the names are."@en ;
        rdfs:domain         cp:CadastralZoning ;
        rdfs:range          gn:GeographicalName ;
        rdfs:subPropertyOf  locn:geographicName ;
        skos:definition     "Name of the cadastral zoning."@en .

cp:CadastralZoning  a          owl:Class ;
        rdfs:comment           "NOTE 1 In the INSPIRE context, cadastral zonings are to be used to carry metadata information and to facilitate portrayal and search of data.\r\n\r\nNOTE 2 Cadastral zonings have generally been defined when cadastral maps were created for the first time.\r\n\r\nEXAMPLE Municipality, section, parish, district, block."@en ;
        rdfs:isDefinedBy       <http://inspire.ec.europa.eu/featureconcept/CadastralZoning> ;
        rdfs:subClassOf        gsp:Feature ;
        iso19150-2:constraint  "zoningLevelHierarchy: /* A lower level cadastral zoning shall be part of an upper level zoning. */ " , "validTo: /* If set, the date validTo shall be equal or later than validFrom. */" , "estimatedAccuracyUoM: /* Value of estimatedAccuracy shall be given in meters. */" , "endLifespanVersion: /* If set, the date endLifespanVersion shall be later than beginLifespanVersion. */" ;
        skos:definition        "Intermediary areas used in order to divide national territory into cadastral parcels."@en .

cp:CadastralZoning.geometry
        a                   owl:ObjectProperty ;
        rdfs:domain         cp:CadastralZoning ;
        rdfs:range          gsp:Geometry ;
        rdfs:subPropertyOf  locn:geometry , gsp:hasDefaultGeometry ;
        skos:definition     "Geometry of the cadastral zoning."@en .

cp:CadastralZoning.nationalCadastalZoningReference
        a                owl:DatatypeProperty ;
        rdfs:comment     "EXAMPLE 03260000AB (France), 30133 (Austria), APD00F (Netherlands)."@en ;
        rdfs:domain      cp:CadastralZoning ;
        rdfs:range       xsd:string ;
        skos:definition  "Thematic identifier at national level, generally the full national code of the cadastral zoning."@en .

cp:CadastralBoundary.parcel
        a                owl:ObjectProperty ;
        rdfs:domain      cp:CadastralBoundary ;
        rdfs:range       cp:CadastralParcel ;
        skos:definition  "The cadastral parcel(s) outlined by this cadastral boundary. A cadastral boundary may outline one or two cadastral parcels."@en .

cp:CadastralBoundary.estimatedAccuracy
        a                owl:DatatypeProperty ;
        rdfs:comment     "NOTE This mean value may come from quality measures on a homogeneous population of cadastral boundaries or from an estimation based on the knowledge of the production processes and of their accuracy."@en ;
        rdfs:domain      cp:CadastralBoundary ;
        rdfs:range       base:Measure ;
        skos:definition  "Estimated absolute positional accuracy of the cadastral boundary in the used INSPIRE coordinate reference system. Absolute positional accuracy is the mean value of the positional uncertainties for a set of positions, where the positional uncertainties are the distance between a measured position and what is considered as the corresponding true position."@en .
